src/BitBlastingCache.v
@@ -1,0 +1,167 @@
+From Coq Require Import Arith ZArith OrderedType.
+From mathcomp Require Import ssreflect ssrfun ssrbool ssrnat eqtype seq.
+From nbits Require Import NBits.
+From ssrlib Require Import Types SsrOrder Var Nats ZAriths Tactics.
+From BitBlasting Require Import Typ TypEnv State QFBV CNF Cache BBExport 
+     AdhereConform BitBlastingCacheDef BitBlastingCacheNewer 
+     BitBlastingCachePreserve BitBlastingCacheCorrect BitBlastingCacheMkEnv 
+     BitBlastingCacheConsistent BitBlastingCacheSat BitBlastingCacheAdhere
+     BitBlastingCacheBound BitBlasting.
+
+Set Implicit Arguments.
+Unset Strict Implicit.
+Import Prenex Implicits.
+
+(* ===== mk_env_cache ===== *)
+
+Lemma init_vm_adhere : 
+  forall te, AdhereConform.adhere init_vm te .
+Proof.
+  done.
+Qed.
+
+Definition init_cache : cache := 
+  {| het := ExpMap.empty (cnf * word);
+     hbt := BexpMap.empty (cnf * literal);
+     cet := ExpMap.empty word;
+     cbt := BexpMap.empty literal |}.
+
+Lemma init_well_formed_cache :
+  Cache.well_formed init_cache.
+Proof.
+  done.
+Qed.
+
+Lemma init_newer_than_cache :
+  newer_than_cache init_gen init_cache.
+Proof.
+  done.
+Qed.
+
+Lemma init_regular :
+  Cache.regular init_env init_cache.
+Proof.
+  done.
+Qed.
+
+Lemma init_correct :
+  forall E s, correct E s init_cache.
+Proof.
+  done.
+Qed.
+
+Lemma init_bound_cache :
+  Cache.bound init_cache init_vm.
+Proof.
+  done.
+Qed.
+
+Definition mk_env_cache (s : SSAStore.t) (e : QFBV.bexp) : env :=
+  let '(m', ca', E', g, cs, lr) := 
+      mk_env_bexp_cache init_vm init_cache s init_env init_gen e in
+  E'.
+
+Lemma mk_env_cache_consistent :
+  forall s e te m ca g cs lr,
+    bit_blast_bexp_cache te init_vm init_cache init_gen e = (m, ca, g, cs, lr) ->
+    AdhereConform.conform_bexp e s te ->
+    QFBV.well_formed_bexp e te ->
+    consistent m (mk_env_cache s e) s.
+Proof.
+  move=> s e te m ca g cs lr Hbb Hcf Hwf. rewrite /mk_env_cache.
+  case Henv: (mk_env_bexp_cache init_vm init_cache s init_env init_gen e) 
+  => [[[[[m' ca'] E'] g'] cs'] lr'].
+  move: (mk_env_bexp_cache_is_bit_blast_bexp_cache Hcf Hwf Henv). 
+  rewrite Hbb. case=> Hm Hca Hg Hcs Hlr.
+  rewrite Hm. apply: (mk_env_bexp_cache_consistent Henv init_newer_than_vm).
+  exact: init_consistent.
+Qed.
+
+Lemma mk_env_cache_tt :
+  forall s e, interp_lit (mk_env_cache s e) lit_tt.
+Proof.
+  move=> s e. rewrite /mk_env_cache.
+  case Henv: (mk_env_bexp_cache init_vm init_cache s init_env init_gen e) 
+  => [[[[[m' ca'] E'] g'] cs'] lr'].
+  rewrite (env_preserve_lit (mk_env_bexp_cache_preserve Henv) init_newer_than_tt).
+  exact: init_tt.
+Qed. 
+
+Lemma mk_env_cache_sat :
+  forall s e te m ca g cs lr,
+    bit_blast_bexp_cache te init_vm init_cache init_gen e = (m, ca, g, cs, lr) ->
+    AdhereConform.conform_bexp e s te ->
+    QFBV.well_formed_bexp e te ->
+    interp_cnf (mk_env_cache s e) cs.
+Proof.
+  move=> s e te m ca g cs lr Hbb Hcf Hwf. 
+  move: (mk_env_cache_tt s e). rewrite /mk_env_cache.
+  case Henv: (mk_env_bexp_cache init_vm init_cache s init_env init_gen e) 
+  => [[[[[m' ca'] E'] g'] cs'] lr'].
+  move: (mk_env_bexp_cache_is_bit_blast_bexp_cache Hcf Hwf Henv).
+  rewrite Hbb; case=> _ _ _ -> _ Htt.
+  exact: (mk_env_bexp_cache_sat Henv init_newer_than_vm init_newer_than_tt 
+                                init_well_formed_cache init_newer_than_cache init_regular).
+Qed.
+
+
+(* ===== mk_state ===== *)
+
+
+
+
+
+(* ===== Soundness and completeness ===== *)
+
+Theorem bit_blast_cache_sound :
+  forall (e : QFBV.bexp) te m' ca' g' cs lr,
+    bit_blast_bexp_cache te init_vm init_cache init_gen e = (m', ca', g', cs, lr) ->
+    QFBV.well_formed_bexp e te ->
+    ~ (sat (add_prelude ([::neg_lit lr]::cs))) ->
+    (forall s,
+        AdhereConform.conform_bexp e s te ->
+        QFBV.eval_bexp e s) .
+Proof.
+  move=> e te m' ca' g' cs lr Hblast Hwf Hsat s Hcf.
+  move: (unsat_implies_valid Hsat) => {Hsat} Hsat.
+  move: (Hsat (mk_env_cache s e)) => {Hsat} Hsat.
+  move: (mk_env_cache_sat Hblast Hcf Hwf) => Hcs. move: (mk_env_cache_tt s e) => Htt.
+  have Hprelude: interp_cnf (mk_env_cache s e) (add_prelude cs)
+    by rewrite add_prelude_expand Hcs Htt.
+  Check bit_blast_bexp_cache_correct.
+  move: (bit_blast_bexp_cache_correct 
+           Hblast Hcf 
+           (mk_env_cache_consistent Hblast Hcf Hwf)
+           Hprelude Hwf
+           init_well_formed_cache 
+           (init_correct (mk_env_cache s e) s)).
+  rewrite /enc_bit. move=> /eqP <-.
+  rewrite Hprelude /= in Hsat. exact: Hsat.
+Qed.
+
+Theorem bit_blast_cache_complete :
+  forall (e : QFBV.bexp) te m' ca' g' cs lr,
+    bit_blast_bexp_cache te init_vm init_cache init_gen e = (m', ca', g', cs, lr) ->
+    QFBV.well_formed_bexp e te ->
+    (forall s, AdhereConform.conform_bexp e s te ->
+               QFBV.eval_bexp e s)
+    ->
+    ~ (sat (add_prelude ([::neg_lit lr]::cs))).
+Proof.
+  move=> e te m' ca' g' cs lr Hblast Hwf He.
+  move=> [E Hcs].
+  rewrite add_prelude_cons in Hcs. move/andP: Hcs => [Hlr Hcs].
+  rewrite add_prelude_expand in Hlr. move/andP: Hlr => [Htt Hlr].
+  rewrite /= interp_lit_neg_lit in Hlr.
+  move : (bit_blast_bexp_cache_adhere (init_vm_adhere te) Hblast) => Hadm' .
+  move : (bit_blast_bexp_cache_bound Hblast init_well_formed_cache init_bound_cache)
+  => Hbound .
+  move : (mk_state_conform_bexp E Hbound Hadm') => Hcf .
+  move : (He (mk_state E m') Hcf) => {He} He .
+  Check bit_blast_bexp_cache_correct.
+  move: (bit_blast_bexp_cache_correct Hblast Hcf (mk_state_consistent E m') 
+                                      Hcs Hwf init_well_formed_cache
+                                      (init_correct E (mk_state E m'))).
+  rewrite /enc_bit => /eqP H. rewrite -H in He.
+  rewrite He in Hlr. exact: not_false_is_true.
+Qed.
