src/BitBlastingCacheBound.v
@@ -1,0 +1,360 @@
+From Coq Require Import Arith ZArith OrderedType.
+From mathcomp Require Import ssreflect ssrfun ssrbool ssrnat eqtype seq.
+From nbits Require Import NBits.
+From ssrlib Require Import Types SsrOrder Var Nats ZAriths Tactics.
+From BitBlasting Require Import Typ TypEnv State QFBV CNF Cache BBExport 
+     AdhereConform BitBlastingCacheDef BitBlastingCachePreserve BitBlastingCacheWF.
+ (* BitBlastingCacheNewer  *)
+ (*     BitBlastingCachePreserve BitBlastingCacheCorrect BitBlastingCacheMkEnv  *)
+ (*     BitBlastingCacheConsistent BitBlastingCacheSat BitBlasting. *)
+
+Set Implicit Arguments.
+Unset Strict Implicit.
+Import Prenex Implicits.
+
+
+Lemma bit_blast_exp_cache_bound_nocache_var :
+  forall (t : SSAVarOrder.t) (te : SSATE.env) (m : SSAVM.t word) 
+         (m' : vm) (ca ca' : cache) (g g' : generator) (cs : cnf) (lrs : word),
+    find_cet (QFBV.Evar t) ca = None ->
+    find_het (QFBV.Evar t) ca = None ->
+    bit_blast_exp_cache te m ca g (QFBV.Evar t) = (m', ca', g', cs, lrs) ->
+    well_formed ca -> bound ca m -> bound_exp (QFBV.Evar t) m' /\ bound ca' m'.
+Proof.
+  move=> v te m m' ca ca' g g' cs lrs Hfcet Hfhet /=.
+  rewrite Hfcet Hfhet.
+  case Hf : (SSAVM.find v m) .
+  - case => <- <- _ _ _ Hwfca Hbcam. 
+    move : (SSAVM.Lemmas.find_some_mem Hf) => Hmem.
+    split; first done.
+    apply bound_add_het. split; last done.
+    by rewrite -bound_add_cet.
+  - dcase (bit_blast_var te g v) => [[[gv csv] lsv] Hbbv] .
+    case => <- <- _ _ _  Hwfca Hbcam.
+    split; first exact: SSAVM.Lemmas.mem_add_eq .
+    apply bound_add_het. split; last exact: SSAVM.Lemmas.mem_add_eq .
+    rewrite -bound_add_cet. exact: (bound_add_find_none lsv Hbcam Hf).
+Qed.
+
+Lemma bit_blast_exp_cache_bound_nocache_const :
+  forall (b : bits) (te : SSATE.env) (m : SSAVM.t word) 
+         (m' : vm) (ca ca' : cache) (g g' : generator) (cs : cnf) (lrs : word),
+    find_cet (QFBV.Econst b) ca = None ->
+    find_het (QFBV.Econst b) ca = None ->
+    bit_blast_exp_cache te m ca g (QFBV.Econst b) = (m', ca', g', cs, lrs) ->
+    well_formed ca -> bound ca m -> bound_exp (QFBV.Econst b) m' /\ bound ca' m'.
+Proof.
+  move=> v te m m' ca ca' g g' cs lrs Hfcet Hfhet /=.
+  rewrite Hfcet Hfhet. case=> <- <- _ _ _ Hwfca Hbcam.
+  split; first done.
+  apply bound_add_het. split; last done.
+  by rewrite -bound_add_cet.
+Qed.
+
+Lemma bit_blast_exp_cache_bound_nocache_extract :
+  forall (i j : nat) (e : QFBV.exp),
+    (forall (te : SSATE.env) (m : SSAVM.t word) (m' : vm) 
+            (ca ca' : cache) (g g' : generator) (cs : cnf) (lrs : word),
+        bit_blast_exp_cache te m ca g e = (m', ca', g', cs, lrs) ->
+        well_formed ca -> bound ca m -> bound_exp e m' /\ bound ca' m') ->
+    forall (te : SSATE.env) (m : SSAVM.t word) (m' : vm) (ca ca' : cache)
+           (g g' : generator) (cs : cnf) (lrs : word),
+      find_cet (QFBV.Eunop (QFBV.Uextr i j) e) ca = None ->
+      find_het (QFBV.Eunop (QFBV.Uextr i j) e) ca = None ->
+      bit_blast_exp_cache te m ca g (QFBV.Eunop (QFBV.Uextr i j) e) =
+      (m', ca', g', cs, lrs) ->
+      well_formed ca ->
+      bound ca m -> bound_exp (QFBV.Eunop (QFBV.Uextr i j) e) m' /\ bound ca' m'.
+Proof.
+(* case => <- _ _ _; exact : (IHe _ _ _ _ _ _ _ Hbbe) . *)
+Admitted.
+
+Lemma bit_blast_exp_cache_bound_nocache_and :
+  forall e1 : QFBV.exp,
+    (forall (te : SSATE.env) (m : SSAVM.t word) (m' : vm) 
+            (ca ca' : cache) (g g' : generator) (cs : cnf) (lrs : word),
+        bit_blast_exp_cache te m ca g e1 = (m', ca', g', cs, lrs) ->
+        well_formed ca -> bound ca m -> bound_exp e1 m' /\ bound ca' m') ->
+    forall e2 : QFBV.exp,
+      (forall (te : SSATE.env) (m : SSAVM.t word) (m' : vm) 
+              (ca ca' : cache) (g g' : generator) (cs : cnf) (lrs : word),
+          bit_blast_exp_cache te m ca g e2 = (m', ca', g', cs, lrs) ->
+          well_formed ca -> bound ca m -> bound_exp e2 m' /\ bound ca' m') ->
+      forall (te : SSATE.env) (m : SSAVM.t word) (m' : vm) (ca ca' : cache)
+             (g g' : generator) (cs : cnf) (lrs : word),
+        find_cet (QFBV.Ebinop QFBV.Band e1 e2) ca = None ->
+        find_het (QFBV.Ebinop QFBV.Band e1 e2) ca = None ->
+        bit_blast_exp_cache te m ca g (QFBV.Ebinop QFBV.Band e1 e2) =
+        (m', ca', g', cs, lrs) ->
+        well_formed ca ->
+        bound ca m -> bound_exp (QFBV.Ebinop QFBV.Band e1 e2) m' /\ bound ca' m'.
+Proof.
+  move=> e1 IH1 e2 IH2 te m m' ca ca' g g' cs lrs Hfcet Hfhet /=.
+  rewrite Hfcet Hfhet.
+  dcase (bit_blast_exp_cache te m ca g e1) => [[[[[m1 ca1] g1] cs1] ls1] Hbbe1].
+  dcase (bit_blast_exp_cache te m1 ca1 g1 e2) => [[[[[m2 ca2] g2] cs2] ls2] Hbbe2].
+  move : (bit_blast_exp_cache_preserve Hbbe1)
+           (bit_blast_exp_cache_preserve Hbbe2) => Hmm1 Hm1m2 .
+  dcase (bit_blast_and g2 ls1 ls2) => [[[gr csr] lsr] Hbbr].
+  case => <- <- _ _ _ Hwfca Hbcam.
+  move: (IH1 _ _ _ _ _ _ _ _ _ Hbbe1 Hwfca Hbcam) => [Hbe1m1 Hbca1m1].
+  move: (bit_blast_exp_cache_well_formed Hbbe1 Hwfca) => Hwfca1.
+  move: (IH2 _ _ _ _ _ _ _ _ _ Hbbe2 Hwfca1 Hbca1m1) => [Hbe2m2 Hbca2m2].
+  have Hbnde : bound_exp e1 m2 && bound_exp e2 m2
+    by rewrite (vm_preserve_bound_exp Hbe1m1 Hm1m2) Hbe2m2.
+  split; first done.
+  apply bound_add_het. split; last done.
+  by rewrite -bound_add_cet. 
+Qed.
+
+Lemma bit_blast_bexp_cache_bound_nocache_conj :
+  forall b1 : QFBV.bexp,
+    (forall (te : SSATE.env) (m : SSAVM.t word) (m' : vm) 
+            (ca ca' : cache) (g g' : generator) (cs : cnf) (lr : literal),
+        bit_blast_bexp_cache te m ca g b1 = (m', ca', g', cs, lr) ->
+        well_formed ca -> bound ca m -> bound_bexp b1 m' /\ bound ca' m') ->
+    forall b2 : QFBV.bexp,
+      (forall (te : SSATE.env) (m : SSAVM.t word) (m' : vm) 
+              (ca ca' : cache) (g g' : generator) (cs : cnf) (lr : literal),
+          bit_blast_bexp_cache te m ca g b2 = (m', ca', g', cs, lr) ->
+          well_formed ca -> bound ca m -> bound_bexp b2 m' /\ bound ca' m') ->
+      forall (te : SSATE.env) (m : SSAVM.t word) (m' : vm) (ca ca' : cache)
+             (g g' : generator) (cs : cnf) (lr : literal),
+        find_cbt (QFBV.Bconj b1 b2) ca = None ->
+        find_hbt (QFBV.Bconj b1 b2) ca = None ->
+        bit_blast_bexp_cache te m ca g (QFBV.Bconj b1 b2) = (m', ca', g', cs, lr) ->
+        well_formed ca -> bound ca m -> 
+        bound_bexp (QFBV.Bconj b1 b2) m' /\ bound ca' m'.
+Proof.
+  move=> e1 IH1 e2 IH2 te m m' ca ca' g g' cs lr Hfcbt Hfhbt /=.
+  rewrite Hfcbt Hfhbt.
+  dcase (bit_blast_bexp_cache te m ca g e1) => [[[[[m1 ca1] g1] cs1] l1] Hbbe1].
+  dcase (bit_blast_bexp_cache te m1 ca1 g1 e2) => [[[[[m2 ca2] g2] cs2] l2] Hbbe2].
+  move : (bit_blast_bexp_cache_preserve Hbbe1)
+           (bit_blast_bexp_cache_preserve Hbbe2) => Hmm1 Hm1m2 .
+  (* dcase (bit_blast_and g2 ls1 ls2) => [[[gr csr] lsr] Hbbr]. *)
+  case => <- <- _ _ _ Hwfca Hbcam.
+  move: (IH1 _ _ _ _ _ _ _ _ _ Hbbe1 Hwfca Hbcam) => [Hbe1m1 Hbca1m1].
+  move: (bit_blast_bexp_cache_well_formed Hbbe1 Hwfca) => Hwfca1.
+  move: (IH2 _ _ _ _ _ _ _ _ _ Hbbe2 Hwfca1 Hbca1m1) => [Hbe2m2 Hbca2m2].
+  have Hbnde : bound_bexp e1 m2 && bound_bexp e2 m2
+    by rewrite (vm_preserve_bound_bexp Hbe1m1 Hm1m2) Hbe2m2.
+  split; first done.
+  apply bound_add_hbt. split; last done.
+  by rewrite -bound_add_cbt. 
+Qed.
+
+
+Corollary bit_blast_exp_cache_bound_cache :
+  forall e te m m' ca ca' g g' cs lrs,
+    bit_blast_exp_cache te m ca g e = (m', ca', g', cs, lrs) ->
+    Cache.well_formed ca -> Cache.bound ca m ->
+    AdhereConform.bound_exp e m' /\ Cache.bound ca' m'
+with
+bit_blast_bexp_cache_bound_cache :
+  forall e te m m' ca ca' g g' cs lr,
+    bit_blast_bexp_cache te m ca g e = (m', ca', g', cs, lr) ->
+    Cache.well_formed ca -> Cache.bound ca m ->
+    AdhereConform.bound_bexp e m' /\ Cache.bound ca' m' .
+Proof .
+  (* bit_blast_exp_cache_bound_cache *)
+  move=> e te m m' ca ca' g g' cs lrs.
+  case Hfcet: (find_cet e ca) => [ls|]. 
+  - rewrite bit_blast_exp_cache_equation Hfcet /=.
+    case=> <- <- _ _ _ Hwfca Hbcam. split; last done.
+    move: (Cache.bound_well_formed_bound_ct Hbcam Hwfca) => [Hct _].
+    by apply (Hct _ _ Hfcet).
+  - case Hfhet: (find_het e ca) => [[csh lsh]|].
+    + rewrite bit_blast_exp_cache_equation Hfcet Hfhet /=. 
+      case=> <- <- _ _ _ Hwfca Hbcam.
+      split; last by rewrite -bound_add_cet.
+      move: Hbcam => [Hht _]. by apply (Hht _ _ _ Hfhet).
+    + move: e te m m' ca ca' g g' cs lrs Hfcet Hfhet.
+      case.
+      * exact: bit_blast_exp_cache_bound_nocache_var.
+      * exact: bit_blast_exp_cache_bound_nocache_const.
+      * elim => [e | e | i j e | n e | n e | n e | n e ];
+                  move: e (bit_blast_exp_cache_bound_cache e).
+        -- admit.
+(* dcase (bit_blast_not g1 ls1) => [[[gr csr] lsr] Hbbr]; *)
+(*         case => <- _ _ _; *)
+(*         exact : (IHe _ _ _ _ _ _ _ Hbbe) . *)
+        -- admit. (* dcase (bit_blast_neg g1 ls1) => [[[gr csr] lsr] Hbbr]; *)
+        (* case => <- _ _ _; *)
+        (* exact : (IHe _ _ _ _ _ _ _ Hbbe) . *)
+        -- exact: bit_blast_exp_cache_bound_nocache_extract. 
+        -- admit. (* case => <- _ _ _; exact : (IHe _ _ _ _ _ _ _ Hbbe) . *)
+        -- admit. (* case => <- _ _ _; exact : (IHe _ _ _ _ _ _ _ Hbbe) . *)
+        -- admit. (* case => <- _ _ _; exact : (IHe _ _ _ _ _ _ _ Hbbe) . *)
+        -- admit.  (* case => <- _ _ _; exact : (IHe _ _ _ _ _ _ _ Hbbe) . *)
+      * elim => e1 e2;
+        move: e1 (bit_blast_exp_cache_bound_cache e1)
+                 e2 (bit_blast_exp_cache_bound_cache e2).
+        -- exact: bit_blast_exp_cache_bound_nocache_and.
+        -- admit. (* dcase (bit_blast_or g2 ls1 ls2) => [[[gr csr] lsr] Hbbr]; *)
+                  (*                               case => <- _ _ _; *)
+                  (*                                         rewrite (vm_preserve_bound_exp (IH0 _ _ _ _ _ _ _ Hbbe0) Hm1m2) *)
+                  (*                                                 (IH1 _ _ _ _ _ _ _ Hbbe1) // . *)
+        -- admit. (*  dcase (bit_blast_xor g2 ls1 ls2) => [[[gr csr] lsr] Hbbr]; *)
+      (* case => <- _ _ _; *)
+      (* rewrite (vm_preserve_bound_exp (IH0 _ _ _ _ _ _ _ Hbbe0) Hm1m2) *)
+      (*         (IH1 _ _ _ _ _ _ _ Hbbe1) // . *)
+        -- admit. (*  dcase (bit_blast_add g2 ls1 ls2) => [[[gr csr] lsr] Hbbr]; *)
+      (* case => <- _ _ _; *)
+      (* rewrite (vm_preserve_bound_exp (IH0 _ _ _ _ _ _ _ Hbbe0) Hm1m2) *)
+      (*         (IH1 _ _ _ _ _ _ _ Hbbe1) // . *)
+        -- admit. (* dcase (bit_blast_sub g2 ls1 ls2) => [[[gr csr] lsr] Hbbr]; *)
+      (* case => <- _ _ _; *)
+      (* rewrite (vm_preserve_bound_exp (IH0 _ _ _ _ _ _ _ Hbbe0) Hm1m2) *)
+      (*         (IH1 _ _ _ _ _ _ _ Hbbe1) // . *)
+        -- admit. (* dcase (bit_blast_mul g2 ls1 ls2) => [[[gr csr] lsr] Hbbr]; *)
+      (* case => <- _ _ _; *)
+      (* rewrite (vm_preserve_bound_exp (IH0 _ _ _ _ _ _ _ Hbbe0) Hm1m2) *)
+      (*         (IH1 _ _ _ _ _ _ _ Hbbe1) // . *)
+        -- admit. (*  case => <- _ _ _; *)
+      (* rewrite (vm_preserve_bound_exp (IH0 _ _ _ _ _ _ _ Hbbe0) Hm1m2) *)
+      (*         (IH1 _ _ _ _ _ _ _ Hbbe1) // . *)
+        -- admit. (* case => <- _ _ _; *)
+      (* rewrite (vm_preserve_bound_exp (IH0 _ _ _ _ _ _ _ Hbbe0) Hm1m2) *)
+      (*         (IH1 _ _ _ _ _ _ _ Hbbe1) // . *)
+        -- admit. (* case => <- _ _ _; *)
+      (* rewrite (vm_preserve_bound_exp (IH0 _ _ _ _ _ _ _ Hbbe0) Hm1m2) *)
+      (*         (IH1 _ _ _ _ _ _ _ Hbbe1) // . *)
+        -- admit. (*  dcase (bit_blast_shl g2 ls1 ls2) => [[[gr csr] lsr] Hbbr]; *)
+      (* case => <- _ _ _; *)
+      (* rewrite (vm_preserve_bound_exp (IH0 _ _ _ _ _ _ _ Hbbe0) Hm1m2) *)
+      (*         (IH1 _ _ _ _ _ _ _ Hbbe1) // . *)
+        -- admit. (*  dcase (bit_blast_lshr g2 ls1 ls2) => [[[gr csr] lsr] Hbbr]; *)
+      (* case => <- _ _ _; *)
+      (* rewrite (vm_preserve_bound_exp (IH0 _ _ _ _ _ _ _ Hbbe0) Hm1m2) *)
+      (*         (IH1 _ _ _ _ _ _ _ Hbbe1) // . *)
+        -- admit. (*  dcase (bit_blast_ashr g2 ls1 ls2) => [[[gr csr] lsr] Hbbr]; *)
+      (* case => <- _ _ _; *)
+      (* rewrite (vm_preserve_bound_exp (IH0 _ _ _ _ _ _ _ Hbbe0) Hm1m2) *)
+      (*         (IH1 _ _ _ _ _ _ _ Hbbe1) // . *)
+        -- admit. (* case => <- _ _ _; *)
+      (* rewrite (vm_preserve_bound_exp (IH0 _ _ _ _ _ _ _ Hbbe0) Hm1m2) *)
+      (*         (IH1 _ _ _ _ _ _ _ Hbbe1) // . *)
+      * move => c e1 e2.
+        move: c (bit_blast_bexp_cache_bound_cache c)
+                e1 (bit_blast_exp_cache_bound_cache e1)
+                e2 (bit_blast_exp_cache_bound_cache e2).
+        admit.
+    (*     dcase (bit_blast_bexp te m g c) => [[[[mc gc] csc] lc] Hbbc] . *)
+    (* dcase (bit_blast_exp te mc gc e0) => [[[[m1 g1] cs1] ls1] Hbb0] . *)
+    (* dcase (bit_blast_exp te m1 g1 e1) => [[[[m2 g2] cs2] ls2] Hbb1] . *)
+    (* dcase (bit_blast_ite g2 lc ls1 ls2) => [[[gr csr] lsr] Hbbr] . *)
+    (* case => <- _ _ _ . *)
+    (* move : (bit_blast_exp_preserve Hbb0) *)
+    (*        (bit_blast_exp_preserve Hbb1) => Hmcm1 Hm1m2 . *)
+    (* move : (vm_preserve_trans Hmcm1 Hm1m2) => Hmcm2 . *)
+    (* rewrite (vm_preserve_bound_bexp (bit_blast_bound_bexp c _ _ _ _ _ _ _ Hbbc) Hmcm2) *)
+    (*         (vm_preserve_bound_exp (IH0 _ _ _ _ _ _ _ Hbb0) Hm1m2) *)
+    (*         (IH1 _ _ _ _ _ _ _ Hbb1) // . *)
+  (* bit_blast_bexp_cache_bound_cache *)
+  move=> e te m m' ca ca' g g' cs lr.
+  case Hfcbt: (find_cbt e ca) => [l|]. 
+  - rewrite bit_blast_bexp_cache_equation Hfcbt /=.
+    case=> <- <- _ _ _ Hwfca Hbcam. split; last done.
+    move: (Cache.bound_well_formed_bound_ct Hbcam Hwfca) => [_ Hct].
+    by apply (Hct _ _ Hfcbt).
+  - case Hfhbt: (find_hbt e ca) => [[csh lh]|].
+    + rewrite bit_blast_bexp_cache_equation Hfcbt Hfhbt /=. 
+      case=> <- <- _ _ _ Hwfca Hbcam.
+      split; last by rewrite -bound_add_cbt.
+      move: Hbcam => [_ Hht]. by apply (Hht _ _ _ Hfhbt).
+    + move: e te m m' ca ca' g g' cs lr Hfcbt Hfhbt.
+      case.
+      * admit.  (* done . *)
+      * admit.  (* done . *)
+      * elim => e1 e2;
+        move: e1 (bit_blast_exp_cache_bound_cache e1)
+                 e2 (bit_blast_exp_cache_bound_cache e2).
+        -- admit.  
+(*       dcase (bit_blast_exp te m g e0) => [[[[m1 g1] cs1] ls1] Hbbe0]; *)
+(*       dcase (bit_blast_exp te m1 g1 e1) => [[[[m2 g2] cs2] ls2] Hbbe1]; *)
+(*       move : (bit_blast_exp_preserve Hbbe1) => Hm1m2 . *)
+
+(* dcase (bit_blast_eq g2 ls1 ls2) => [[[g'0 cs] r] Hbbr]; case => <- _ _ _; *)
+(*       rewrite (vm_preserve_bound_exp (bit_blast_bound_exp _ _ _ _ _ _ _ _ Hbbe0) Hm1m2) *)
+(*               (bit_blast_bound_exp _ _ _ _ _ _ _ _ Hbbe1) // . *)
+        -- admit. (* dcase (bit_blast_ult g2 ls1 ls2) => [[[g'0 cs] r] Hbbr]; case => <- _ _ _; *)
+      (* rewrite (vm_preserve_bound_exp (bit_blast_bound_exp _ _ _ _ _ _ _ _ Hbbe0) Hm1m2) *)
+      (*         (bit_blast_bound_exp _ _ _ _ _ _ _ _ Hbbe1) // . *)
+        -- admit. (* dcase (bit_blast_ule g2 ls1 ls2) => [[[g'0 cs] r] Hbbr]; case => <- _ _ _; *)
+      (* rewrite (vm_preserve_bound_exp (bit_blast_bound_exp _ _ _ _ _ _ _ _ Hbbe0) Hm1m2) *)
+      (*         (bit_blast_bound_exp _ _ _ _ _ _ _ _ Hbbe1) // . *)
+        -- admit. (* dcase (bit_blast_ugt g2 ls1 ls2) => [[[g'0 cs] r] Hbbr]; case => <- _ _ _; *)
+      (* rewrite (vm_preserve_bound_exp (bit_blast_bound_exp _ _ _ _ _ _ _ _ Hbbe0) Hm1m2) *)
+      (*         (bit_blast_bound_exp _ _ _ _ _ _ _ _ Hbbe1) // . *)
+        -- admit. (*  dcase (bit_blast_uge g2 ls1 ls2) => [[[g'0 cs] r] Hbbr]; case => <- _ _ _; *)
+      (* rewrite (vm_preserve_bound_exp (bit_blast_bound_exp _ _ _ _ _ _ _ _ Hbbe0) Hm1m2) *)
+      (*         (bit_blast_bound_exp _ _ _ _ _ _ _ _ Hbbe1) // . *)
+        -- admit. (*  dcase (bit_blast_slt g2 ls1 ls2) => [[[g'0 cs] r] Hbbr]; case => <- _ _ _; *)
+      (* rewrite (vm_preserve_bound_exp (bit_blast_bound_exp _ _ _ _ _ _ _ _ Hbbe0) Hm1m2) *)
+      (*         (bit_blast_bound_exp _ _ _ _ _ _ _ _ Hbbe1) // . *)
+        -- admit. (*  dcase (bit_blast_sle g2 ls1 ls2) => [[[g'0 cs] r] Hbbr]; case => <- _ _ _; *)
+      (* rewrite (vm_preserve_bound_exp (bit_blast_bound_exp _ _ _ _ _ _ _ _ Hbbe0) Hm1m2) *)
+      (*         (bit_blast_bound_exp _ _ _ _ _ _ _ _ Hbbe1) // . *)
+        -- admit. (*  dcase (bit_blast_sgt g2 ls1 ls2) => [[[g'0 cs] r] Hbbr]; case => <- _ _ _; *)
+      (* rewrite (vm_preserve_bound_exp (bit_blast_bound_exp _ _ _ _ _ _ _ _ Hbbe0) Hm1m2) *)
+      (*         (bit_blast_bound_exp _ _ _ _ _ _ _ _ Hbbe1) // . *)
+        -- admit. (*  dcase (bit_blast_sge g2 ls1 ls2) => [[[g'0 cs] r] Hbbr]; case => <- _ _ _; *)
+      (* rewrite (vm_preserve_bound_exp (bit_blast_bound_exp _ _ _ _ _ _ _ _ Hbbe0) Hm1m2) *)
+      (*         (bit_blast_bound_exp _ _ _ _ _ _ _ _ Hbbe1) // . *)
+        -- admit. (*  dcase (bit_blast_uaddo g2 ls1 ls2) => [[[g'0 cs] r] Hbbr]; case => <- _ _ _; *)
+      (* rewrite (vm_preserve_bound_exp (bit_blast_bound_exp _ _ _ _ _ _ _ _ Hbbe0) Hm1m2) *)
+      (*         (bit_blast_bound_exp _ _ _ _ _ _ _ _ Hbbe1) // . *)
+        -- admit. (*  dcase (bit_blast_usubo g2 ls1 ls2) => [[[g'0 cs] r] Hbbr]; case => <- _ _ _; *)
+      (* rewrite (vm_preserve_bound_exp (bit_blast_bound_exp _ _ _ _ _ _ _ _ Hbbe0) Hm1m2) *)
+      (*         (bit_blast_bound_exp _ _ _ _ _ _ _ _ Hbbe1) // . *)
+        -- admit. (*  dcase (bit_blast_umulo g2 ls1 ls2) => [[[g'0 cs] r] Hbbr]; case => <- _ _ _; *)
+      (* rewrite (vm_preserve_bound_exp (bit_blast_bound_exp _ _ _ _ _ _ _ _ Hbbe0) Hm1m2) *)
+      (*         (bit_blast_bound_exp _ _ _ _ _ _ _ _ Hbbe1) // . *)
+        -- admit. (*  dcase (bit_blast_saddo g2 ls1 ls2) => [[[g'0 cs] r] Hbbr]; case => <- _ _ _; *)
+      (* rewrite (vm_preserve_bound_exp (bit_blast_bound_exp _ _ _ _ _ _ _ _ Hbbe0) Hm1m2) *)
+      (*         (bit_blast_bound_exp _ _ _ _ _ _ _ _ Hbbe1) // . *)
+        -- admit. (* dcase (bit_blast_ssubo g2 ls1 ls2) => [[[g'0 cs] r] Hbbr]; case => <- _ _ _; *)
+      (* rewrite (vm_preserve_bound_exp (bit_blast_bound_exp _ _ _ _ _ _ _ _ Hbbe0) Hm1m2) *)
+      (*         (bit_blast_bound_exp _ _ _ _ _ _ _ _ Hbbe1) // . *)
+        -- admit. (*  dcase (bit_blast_smulo g2 ls1 ls2) => [[[g'0 cs] r] Hbbr]; case => <- _ _ _; *)
+      (* rewrite (vm_preserve_bound_exp (bit_blast_bound_exp _ _ _ _ _ _ _ _ Hbbe0) Hm1m2) *)
+      (*         (bit_blast_bound_exp _ _ _ _ _ _ _ _ Hbbe1) // . *)
+      * admit. (*  move => c IHc te m m' g g' cs' lrs' . *)
+    (* dcase (bit_blast_bexp te m g c) => [[[[m1 g1] cs1] l1] Hbbc] . *)
+    (* case => <- _ _ _ ; rewrite (IHc _ _ _ _ _ _ _ Hbbc) // . *)
+      * move => b1 b2;
+        move: b1 (bit_blast_bexp_cache_bound_cache b1)
+                 b2 (bit_blast_bexp_cache_bound_cache b2).
+        exact: bit_blast_bexp_cache_bound_nocache_conj.
+      * admit. (*  move => b0 IH0 b1 IH1 te m m' g g' cs' lrs' . *)
+    (* dcase (bit_blast_bexp te m g b0) => [[[[m1 g1] cs1] l1] Hbb0] . *)
+    (* dcase (bit_blast_bexp te m1 g1 b1) => [[[[m2 g2] cs2] l2] Hbb1] . *)
+    (* case => <- _ _ _ . *)
+    (* move : (bit_blast_bexp_preserve Hbb1) => Hm1m2 . *)
+    (* rewrite (vm_preserve_bound_bexp (IH0 _ _ _ _ _ _ _ Hbb0) Hm1m2) *)
+    (*         (IH1 _ _ _ _ _ _ _ Hbb1) // . *)
+Admitted.
+
+
+Corollary bit_blast_exp_cache_bound :
+  forall e te m m' ca ca' g g' cs lrs,
+    bit_blast_exp_cache te m ca g e = (m', ca', g', cs, lrs) ->
+    Cache.well_formed ca -> Cache.bound ca m ->
+    AdhereConform.bound_exp e m'.
+Proof.
+  move=> e te m m' ca ca' g g' cs lrs Hbb Hwfca Hbcam.
+  move: (bit_blast_exp_cache_bound_cache Hbb Hwfca Hbcam) => [Hbe _].
+  done.
+Qed.
+
+Corollary bit_blast_bexp_cache_bound :
+  forall e te m m' ca ca' g g' cs lr,
+    bit_blast_bexp_cache te m ca g e = (m', ca', g', cs, lr) ->
+    Cache.well_formed ca -> Cache.bound ca m ->
+    AdhereConform.bound_bexp e m'.
+Proof.
+  move=> e te m m' ca ca' g g' cs lr Hbb Hwfca Hbcam.
+  move: (bit_blast_bexp_cache_bound_cache Hbb Hwfca Hbcam) => [Hbe _].
+  done.
+Qed.
